SP1Chips/Sub/U16Composition.lean
@@ -8,12 +8,10 @@ namespace Sub
 
 section u16_composition
 
-variable
+set_option maxHeartbeats 400000 in
+theorem u16_composition 
   (Main : Vector (Fin BB) 33)
   (cstrs : (constraints Main).allHold)
-
-set_option maxHeartbeats 400000 in
-def u16_composition 
   : (constraints Main).U16CompProp
   := by
     simp [SP1Constraint.toU16CompProp, constraints, List.Forall, SubOperation.constraints, CPUState.constraints, RTypeReader.constraints]
@@ -62,6 +60,8 @@ def u16_composition
         extract_from_and reader_cstrs'
       refine ⟨⟨h_is_u64 0, h_is_u64 1, h_is_u64 2, h_is_u64 3⟩, ?_⟩
       extract_from_and reader_cstrs'
+
+#print axioms u16_composition
 
 end u16_composition
 
